1. $\hspace{1cm} sin^2 \theta + cos^2 \theta = 1$
2. $\hspace{1.5cm} 1 + cot^2 \theta = cosec^2 \theta$
3.  $\hspace{1.5cm} 1 + tan^2 \theta = sec^2 \theta$

### Trignometric Formulae

$sin(x+y) = \sin{x}.\cos{y} + \cos{x}.sin{y}$
$sin(x-y) = \sin{x}.\cos{y} - \cos{x}.\sin{y}$
$cos(x+y) = \cos{x}.\cos{y} - \sin{x}.\sin{y}$
$\cos(x+y) = \cos{x}.\cos{y} + \sin{x}.\sin{y}$

$\tan(x+y) = \frac{\tan{x} + \tan{y}}{1 - \tan{x}\tan{y}}$

$\tan(x-y) = \frac{\tan{x} - \tan{y}}{1+ \tan{x}.\tan{y}}$

-------

$\sin{2x} = 2\sin{x}.\cos{x} = frac{2\tan{x}}{1 + \tan^2{x}}$

$cos2x = 2cos^2x -1 = 1 - 2sin^2x = cos^2x - sin^2x = \frac{1-\tan^2{x}}{1+ \tan^2{x}}$

$\tan{2x} =  \frac{2\tan{x}}{1- \tan^2{x}}$

----
$\sin^3{x} = \frac{3\sin{x} - \sin{3x}}{4}$

$\cos^3{x} = \frac{3\cos{x} + \cos{3x}}{4}$
------

$1 + \cos{2x} = 2\cos^2{x}$
$1-  \cos{2x} = 2\sin^2{x}$
---

$\sin{3x} = 3\sin{x} - 4\sin^3{x}$
$\cos{3x} = 4cos^3{x} - 3\cos{x}$
$\tan{3x} =  \frac{3\tan{x} - \tan^3{x}}{1 - 3\tan^2{x}}$
------

##### Transformation Formulae

$\sin(x+y) + \sin(x-y) = 2.\sin{x}.\cos{y}$
$\sin(x+y) - \sin(x-y) = 2.\cos{x}.\sin{y}$
$\cos(x+y) + \cos(x-y) = 2.\cos{x}.\cos{y}$
$\cos(x+y) - \cos(x-y) = 2.\sin{x}.\sin{y}$

$\sin{N} + \sin{Z} = 2\sin{\frac{N+Z}{2}} \times cos{\frac{N-Z}{2}}$

$\sin{N} - \sin{Z} = 2\cos{\frac{N+Z}{2}} \times sin{\frac{N-Z}{2}}$

$\cos{N} + \cos{Z} = 2\cos{\frac{N+Z}{2}} \times cos{\frac{N-Z}{2}}$

$\cos{N} - \cos{Z} = -2\sin{\frac{N+Z}{2}} \times sin{\frac{N-Z}{2}}$

-----

$\sin(A+B).\sin(A-B) = \sin^2{A} - \sin^2{B} = \cos^2{B} - \cos^2{A}$
$\cos(A+B).\cos(A-B) = \cos^2{A} - \sin^2{B} = \cos^2{B} - \sin^2{A}$

$\sin(A+B+C) = \sin{A}.\cos{B}.\cos{C} + \cos{A}.\sin{B}.\cos{C} + \cos{A}.\cos{B}.\sin{C} - \sin{A}.\sin{B}.\sin{C}$

$\cos(A+B+C) = \cos{A}.\cos{B}.\cos{C} - \cos{A}.\sin{B}.\sin{C} + \sin{A}.\cos{B}.\sin{C} - \sin{A}.\sin{B}.\cos{C}$

$\tan(A+B+C) = \frac{\tan{A} + \tan{B} + \tan{C} - \tan{A}.\tan{B}.\tan{C}}{1 - (\tan{A}.\tan{B} + \tan{B}.\tan{C} + \tan{C}.\tan{A})}$

- If A+B = $\pi$, then

$\sin{A} = \sin{B}$
$\cos{A} = - \cos{B}$
$\tan{A} = - \tan{B}$

- If A+B = $2\pi$, then

$\sin{A} = -\sin{B}$
$\cos{A} = \cos{B}$
$\tan{A} = - \tan{B}$

----

$\tan(\frac{\pi}{4} + x) =  \frac{1+ \tan{x}}{ 1 - \tan{x}}$

$\tan(\frac{\pi}{4} - x) =  \frac{1- \tan{x}}{ 1 + \tan{x}}$

-----------------

| | | |
|--|--|
| $\sin(- \theta) = - \sin{\theta}$ | $\csc(-\theta) = \csc{\theta}$  |
| $\cos(- \theta) = \cos{\theta}$  | $\sec(- \theta) = \sec{\theta}$ |
| $\tan(- \theta) = - \tan{\theta}$ | $\cot(- \theta) = - \cot(\theta)$ |

|  |  |  |  |
|--|--|--|--|
| $\sin(90- \theta) = \cos{\theta}$ | $\csc(90-\theta) = \sec{\theta}$ | $\sin(90+ \theta) = \cos{\theta}$ | $\csc(90+\theta) = \sec{\theta}$  | 
| $\cos(90- \theta) = \sin{\theta}$ | $\sec(90- \theta) = \csc{\theta}$ | $\cos(90+ \theta) = - \sin{\theta}$  | $\sec(90+ \theta) = -\csc{\theta}$ | 
| $\tan(90- \theta) = \cot{\theta}$ | $\cot(90- \theta) = \tan{\theta}$ | $\tan(90+ \theta) = - \cot{\theta}$ | $\cot(90+ \theta) = - \tan(\theta)$ |

---------------

## Inverse Trignometric Functions

| Function | Domain | Range   |
| -- | -- | -- |
| $y = \sin^-1{x}$| [-1, 1] | $[ -\frac{\pi}{2} , \frac{\pi}{2}]$|
| $y = \cos^-1{x}$| [-1, 1] | $[ 0 , \pi]$|
| $y = \tan^-1{x}$| R | $] -\frac{\pi}{2} , \frac{\pi}{2}[$|
| $y = \csc^-1{x}$| R - $]-1, 1[$ | $[ -\frac{\pi}{2} , \frac{\pi}{2}] - \{0\}$ |
| $y = \sec^-1{x}$| R - $]-1, 1[$ | $[ 0 , \pi] - \{\frac{\pi}{2}\}$ |
| $y = \cot^-1{x}$ | R | $[ 0 , \pi]$|


----------

$\sin^{-1}(\sin{x}) = x \hspace{0.5cm} or \hspace{0.5cm}\sin(\sin^{-1}{x}) = x$
$\cos^{-1}(\cos{x}) = x \hspace{0.5cm} or \hspace{0.5cm}\cos(\cos^{-1}{x}) = x$
$\tan^{-1}(\tan{x}) = x \hspace{0.5cm} or \hspace{0.5cm}\tan(\tan^{-1}{x}) = x$

and similar for cosec, sec & cot.

----

$\sin^{-1}(-x) = - \sin^{-1}(x)$
$\cos^{-1}(-x) = \pi - \cos^{-1}(x)$
$\tan^-1(-x) = - \tan^{-1}(x)$
$\csc^{-1}(-x) = - \csc^{-1}(x)$
$\sec^{-1}(-x) = \pi - \sec^{-1}(x)$
$\cot^{-1}(-x) = \pi - \cot^{-1}(x)$

-----

$\sin^{-1}(\frac{1}{x}) = \csc^-1{x}$                      $\csc^{-1}(\frac{1}{x}) = \sin^-1{x}$  

$\sin^{-1}(\frac{1}{x}) = \csc^-1{x}$                     $\sec^{-1}(\frac{1}{x}) = \cos^-1{x}$                    

$\tan^{-1}(\frac{1}{x}) = \cot^-1{x}$                    $\cot^{-1}(\frac{1}{x}) = \tan^-1{x}$


-----

$\sin^{-1}{x} + \cos^{-1}{x} = \frac{\pi}{2}$
$\sec^{-1}{x} + \csc^{-1}{x} = \frac{\pi}{2}$
$\tan^{-1}{x} + \cot^{-1}{x} = \frac{\pi}{2}$

---------------

$\sin^{-1}{x} \pm \sin^{-1}{y} = \sin^{-1}(x + \sqrt{1 - y^2} \pm y.\sqrt{1-x^2})$

$\cos^{-1}{x} \pm \cos^{-1}{y} = \cos^{-1}(xy \mp \sqrt{1 - x^2} \times \sqrt{1-y^2})$

$\tan^{-1}{x} + \tan^{-1}{y} = \tan^{-1}(\frac{x+y}{1-xy}))$                        if, xy < 1

$\tan^{-1}{x} - \tan^{-1}{y} = \tan^{-1}(\frac{x-y}{1+xy}))$                        if, xy > -1

$2\tan^{-1}{x} = \sin^{-1}(\frac{2x}{1 + x^2}) = \cos^{-1}(\frac{1-x^2}{1 + x^2}) = \tan^{-1}(\frac{2x}{1-x^2})$

$3\tan^{-1}{x} = \tan^{-1}(\frac{3x - x^3}{1 - 3x^2})$

----

#### Substitutions to simplify Inverse Trignometric Functions
For:Put

$\sqrt{1-x^2} : x = \sin{\theta}/\cos{\theta}$
$\sqrt{x^2 -1}: x = \sec{\theta}/\csc{\theta}$
$\sqrt{1+x^2} or \sqrt{x^2 +1} : x = \tan{\theta}/\cot{\theta}$

----

$\sqrt{1+x} \hspace{0.5cm} or \hspace{0.5cm} \sqrt{1-x} \hspace{0.5cm} \text{ (or both) }: x = \cos{\theta}/ -cos{\theta}$
$\sqrt{1+x^2} \hspace{0.5cm} or \hspace{0.5cm} \sqrt{1-x^2} \hspace{0.5cm} \text{ (or both) }: x = \cos{\theta}/ -cos{\theta}$

$a^2-x^2 \hspace{0.5cm}; \hspace{0.5cm} \sqrt{a^2-x^2} \hspace{0.5cm} : \hspace{0.5cm} x = a.\sin{\theta} / a.\cos{\theta}$
$a^2+x^2 \hspace{0.5cm}; \hspace{0.5cm} \sqrt{a^2+x^2} \hspace{0.5cm} : \hspace{0.5cm} x = a.\tan{\theta} / a.\cot{\theta}$
$x^2-a^2 \hspace{0.5cm}; \hspace{0.5cm} \sqrt{x^2 - a^2} \hspace{0.5cm} : \hspace{0.5cm} x=a.\sec{\theta} / a.\csc{\theta}$

$a \pm x \hspace{0.5cm} :  \hspace{0.5cm} a.\cos{\theta} / a . \cos{2\theta}$

----

$\sqrt{a^4 - x^4} : x^2 = a^2.\sin{\theta} / a^2.\cos{\theta}$
$\sqrt{x^4 - a^4} : x^2 = a^2.\sec{\theta} / a^2.\csc{\theta}$
$\sqrt{a^4 + x^4} : x^2 = a^2.\tan{\theta} / a^2.\cot{\theta}$

$\sqrt{1 - a^2.x^2} : ax = \sin{\theta} / \cos{\theta}$
$\sqrt{1 + a^2.x^2} : ax = \tan{\theta} / \cot{\theta}$
$\sqrt{a^2.x^2 -1} : ax = \sec{\theta} / \csc{\theta}$

$\frac{1-x^2}{1 + x^2} \hspace{0.5cm} ; \hspace{0.5cm} \frac{2x}{1 + x^2} \hspace{0.5cm} ; \hspace{0.5cm} \frac{2x}{1- x^2} : x = \tan{\theta}$

$\frac{3x - x^3}{ 1 - 3x^2}: x = \tan{\theta}$

$\sin^{-1}{\sqrt{\frac{1 + x^2}{2}}} : x^2 = -\cos{\theta}$
$\cos^{-1}{\sqrt{\frac{1 + x^2}{2}}} : x^2 = \cos{\theta}$

$\sqrt{\frac{x}{a+x}} :  x = a.\tan^2{\theta} / a.\cot^2{\theta}$

$\frac{1}{x + \sqrt{a^2 - x^2}} :  x = a.\sin{\theta}$

$\frac{x^4}{\sqrt{a^2 - x^2}} : x = a.\sin{\theta}$

------------------


